On the way to adapting Hashed El Gamal.
CDH in 1.0, with bug workarounds galore!

examples/CDH.ec
@@ -5,39 +5,30 @@ require import FSet.
 
 (** Minimalist group theory with only needed components *)
 theory Group.
-
   type group.
 
-  const q : int.
+  const q: int.
+  const g: group.
+  axiom q_pos: 0 < q.
 
-  const g : group.
+  op ( * ): group -> group -> group.
+  op ( ^ ): group -> int -> group.
 
-  axiom q_pos  : 0 < q.
-
-  op ( * ) : group -> group -> group.
-
-  op ( ^ ) : group -> int -> group.
-
-  axiom pow_mult (x y:int) : (g ^ x) ^ y = g ^ (x * y).
- 
-  axiom pow_plus (x y:int) : (g ^ x) * (g ^ y) = g ^ (x + y).
-
+  axiom pow_mult (x y:int): (g ^ x) ^ y = g ^ (x * y). 
+  axiom pow_plus (x y:int): (g ^ x) * (g ^ y) = g ^ (x + y).
 end Group.
-
 
 (** Computational Diffie-Hellman problem *)
 theory CDH.
-
   import Group.
 
   module type Adversary = {
-    fun solve(gx gy:group) : group {*}
+    proc solve(gx gy:group): group
   }.
 
   module CDH (A:Adversary) = {
-    fun main() : bool = {
-      var x, y : int;
-      var r : group;
+    proc main(): bool = {
+      var x, y, r;
 
       x = $[0..q-1];
       y = $[0..q-1];
@@ -45,25 +36,21 @@ theory CDH.
       return (r = g ^ (x * y));
     }
   }.
-
 end CDH.
-
 
 (** Set version of the Computational Diffie-Hellman problem *)
 theory Set_CDH.
-
   import Group.
 
-  const n : int.
+  const n: int.
 
   module type Adversary = {
-    fun solve(gx:group, gy:group) : group set {*}
+    proc solve(gx:group, gy:group): group set
   }.
 
   module SCDH (B:Adversary) = {
-    fun main() : bool = {
-      var x, y : int;
-      var s : group set;
+    proc main(): bool = {
+      var x, y, s;
 
       x = $[0..q-1];
       y = $[0..q-1];
@@ -72,10 +59,9 @@ theory Set_CDH.
     }
   }.
 
-  module CDH_from_SCDH (A:Adversary) : CDH.Adversary = {
-    fun solve(gx:group, gy:group) : group = {
-      var s : group set;
-      var x : group;
+  module CDH_from_SCDH (A:Adversary): CDH.Adversary = {
+    proc solve(gx:group, gy:group): group = {
+      var s, x;
 
       s = A.solve(gx, gy);
       x = $Duni.duni s;
@@ -83,102 +69,97 @@ theory Set_CDH.
     }
   }.
 
-
   (** Naive reduction to CDH *)
-
   (* Useful lemmas on reals, maybe move to Real.ec *)
-  lemma nosmt le_compat_r (w x y: real) : 0%r < w => x * w <= y * w => x <= y 
+  lemma nosmt le_compat_r (w x y:real): 0%r < w => x * w <= y * w => x <= y 
   by [].
 
-  lemma nosmt inv_le (x y:real) : 0%r < x => 0%r < y => y <= x => inv x <= inv y.
+  lemma nosmt inv_le (x y:real): 0%r < x => 0%r < y => y <= x => inv x <= inv y.
   proof.
-    intros _ _ _.
+    move=> _ _ _.
     apply (le_compat_r x); first trivial.
     apply (le_compat_r y); first trivial.
-    cut H : ((x * inv x) * y <= (y * inv y) * x); last smt.
+    cut H: ((x * inv x) * y <= (y * inv y) * x); last smt.
     rewrite (Inverse y _); first smt.
     by rewrite (Inverse x _); smt.
   qed.
 
-  lemma div_le (x y:real) : 
+  lemma div_le (x y:real): 
     0%r < x => 0%r < y => y <= x => 1%r / x <= 1%r / y .
-  proof.
-    by progress; cut X := inv_le x y; smt.
-  qed.
+  proof. by progress; cut X:= inv_le x y; smt. qed.
 
-  lemma mu_duni_mem (s:'a set) (x:'a) :
+  lemma mu_duni_mem (s:'a set) (x:'a):
     mem x s => 1%r / (card s)%r <= mu (Duni.duni s) ((=) x).
-  proof.
-    by intros _; rewrite Duni.mu_def; smt.
-  qed.
+  proof. by intros _; rewrite Duni.mu_def; smt. qed.
 
-  module SCDH' (A:Adversary) = {
-    var x, y : int
+  section.
+    declare module A: Adversary.
 
-    fun aux() : group set = {
-      var s : group set;
-      x = $[0..q-1];
-      y = $[0..q-1];
-      s = A.solve(g ^ x, g ^ y);
-      return s;
-    }
+    local module SCDH' = {
+      var x, y: int
 
-    fun main() : bool = {
-      var z : group;
-      var s : group set;
-      s = aux();
-      z = $Duni.duni s;
-      return z = g ^ (x * y);
-    }
-  }.
+      proc aux(): group set = {
+        var s;
 
-  lemma Reduction (A <: Adversary {SCDH'}) &m :
-    0 < n =>
-    exists (B <: CDH.Adversary), 
-      1%r / n%r * Pr[SCDH(A).main() @ &m : res] <=
-      Pr[CDH.CDH(B).main() @ &m : res]. 
-  proof.
-   intros n_pos; exists (CDH_from_SCDH(A)).
-   apply (Trans _ Pr[SCDH'(A).main() @ &m : res]); first last.
-     equiv_deno (_ : true ==> ={res}) => //.
-     fun; inline CDH_from_SCDH(A).solve SCDH'(A).aux.
-     by wp; rnd; wp; call (_:true); wp; do rnd.
-   
-     bdhoare_deno (_ : true ==> _) => //.
-     fun. 
-     seq 1 : (mem (g ^ (SCDH'.x * SCDH'.y)) s /\ card s <= n)
-             Pr[SCDH(A).main() @ &m: res]
-             (1%r / n%r)
-             (1%r - Pr[SCDH(A).main() @ &m: res])
-             0%r => //. 
-       conseq (_ : _ : = (Pr[SCDH(A).main() @ &m : res])).
-       call (_ : true ==> mem (g ^ (SCDH'.x * SCDH'.y)) res /\ card res <= n) => //.
-       bypr; progress.
-       equiv_deno (_: 
-         true ==> 
-         (mem (g ^ (SCDH'.x * SCDH'.y)) res /\ card res <= n){1} = res{2}) => //.
-       fun *; inline SCDH(A).main SCDH'(A).aux; wp.
-       by call (_:true); do rnd; skip; smt.
-       
-       rnd ((=) (g ^ (SCDH'.x * SCDH'.y))).
-       by skip => &m1 H1; split => //; rewrite Duni.mu_def; smt.
-  qed.  
+        x = $[0..q-1];
+        y = $[0..q-1];
+        s = A.solve(g ^ x, g ^ y);
+        return s;
+      }
 
+      proc main(): bool = {
+        var z, s;
+
+        s = aux();
+        z = $Duni.duni s;
+        return z = g ^ (x * y);
+      }
+    }.
+
+    lemma Reduction &m:
+      0 < n =>
+      1%r / n%r * Pr[SCDH(A).main() @ &m: res]
+      <= Pr[CDH.CDH(CDH_from_SCDH(A)).main() @ &m: res].
+    proof.
+      move=> n_pos.
+      apply (Trans _ Pr[SCDH'.main() @ &m: res]); first last.
+        byequiv (_: ={glob A} ==> ={res})=> //.
+        proc; inline CDH_from_SCDH(A).solve SCDH'.aux.
+        by wp; rnd; wp; call (_: true); wp; do rnd.
+      byphoare (_: (glob A) = (glob A){m} ==> _)=> //.
+      pose d:= 1%r/n%r * Pr[SCDH(A).main() @ &m: res]; conseq (_: _: >= d). (* bug *)
+      pose d':= Pr[SCDH(A).main() @ &m: res].
+      proc.
+      seq  1: (mem (g ^ (SCDH'.x * SCDH'.y)) s /\ card s <= n)
+              d' (1%r / n%r) _ 0%r => //. 
+        conseq (_ : (glob A) = (glob A){m} : = d').
+        call (_: (glob A) = (glob A){m} ==> mem (g ^ (SCDH'.x * SCDH'.y)) res /\ card res <= n) => //.
+        bypr; progress; rewrite /d'.
+        byequiv (_: ={glob A} ==>
+                    (mem (g ^ (SCDH'.x * SCDH'.y)) res /\
+                     card res <= n){1} = res{2}) => //.
+        proc*; inline SCDH(A).main SCDH'.aux; wp.
+        by call (_: true); do rnd.
+      rnd ((=) (g ^ (SCDH'.x * SCDH'.y))).
+      skip; progress; rewrite Duni.mu_def; first smt.
+      cut ->: card (filter ((=) (g ^ (SCDH'.x * SCDH'.y))) s){hr} = 1 by smt.
+      by apply div_le; expect 3 smt.
+    qed.  
+  end section.
+
+(*
   (** Shoup's reduction to CDH -- would be nice to prove a bound *)
-
   module CDH_from_SCDH_Shoup (A:Adversary, B:Adversary) : CDH.Adversary = {
-    fun solve(gx:group, gy:group) : group = {
-      var a, b : int;
-      var s1, s2 : group set;
-      var r : group;
+    proc solve(gx:group, gy:group) : group = {
+      var a, b, s1, s2, r;
 
       s1 = A.solve(gx, gy);
       a = $[0..q-1];
       b = $[0..q-1];
       s2 = B.solve(gx ^ a * g ^ b, g ^ b);    
-      r = pick (filter (lambda (z:group), mem (z ^ a * gy ^ b) s2) s1);
+      r = pick (filter (fun (z:group), mem (z ^ a * gy ^ b) s2) s1);
       return r;
     }
   }.
-
+*)
 end Set_CDH.
